---
layout: default
---

**goal**

map $$x$$ from the interval $$[x_0,x_1]$$ to the interval $$[y_0,y_1]$$

**solution**

For a linear mapping

$$y = m x + b$$

$$y_0 = m x_0 + b$$

$$y_1 = m x_1 + b$$

subtracting

$$y_1 - y_0 = m (x_1 - x_0)$$

$$m = \frac{y_1 - y_0}{x_1 - x_0}$$

solve for $$b$$

$$y_0 = \frac{y_1 - y_0}{x_1 - x_0} x_0 + b$$

$$b = y_0 - \frac{y_1 - y_0}{x_1 - x_0} x_0$$

finally

$$
y = \frac{y_1 - y_0}{x_1 - x_0} x + y_0 - \frac{y_1 - y_0}{x_1 - x_0} x_0
$$

$$
y = \frac{y_1 - y_0}{x_1 - x_0} (x - x_0) + y_0
$$


